Basic_Assn.thy
@@ -47,4 +47,310 @@ lemma prod_assn_cong[fundef_cong]:
   apply (cases p; cases pi)
   by auto
 
+(*
+subsection \<open>Four-List-Assn\<close>
+
+
+fun four_list_assn :: "('a \<Rightarrow> 'b \<Rightarrow> 'c \<Rightarrow> 'd \<Rightarrow> assn) \<Rightarrow> 'a list \<Rightarrow> 'b list \<Rightarrow> 'c list \<Rightarrow> 'd list \<Rightarrow> assn" where
+  "four_list_assn P [] [] [] [] = emp"
+| "four_list_assn P (a#as) (b#bs) (c#cs) (d#ds) = P a b c d * four_list_assn P as bs cs ds"
+| "four_list_assn _ _ _ _ _ = false"
+
+lemma four_list_assn_aux_simps[simp]:
+  "four_list_assn P [] l' l'' l''' = (\<up>(l'=[] \<and> l''=[] \<and> l'''=[]))"
+  "four_list_assn P l [] l'' l''' = (\<up>(l=[] \<and> l''=[] \<and> l'''=[]))"
+  "four_list_assn P l l' [] l''' = (\<up>(l=[] \<and> l'=[] \<and> l'''=[]))"
+  "four_list_assn P l l' l'' [] = (\<up>(l=[] \<and> l'=[] \<and> l''=[]))"
+  subgoal by (cases l; cases l'; cases l''; cases l''') auto
+  subgoal by (cases l; cases l'; cases l''; cases l''') auto
+  subgoal by (cases l; cases l'; cases l''; cases l''') auto
+  subgoal by (cases l; cases l'; cases l''; cases l''') auto
+  done
+
+lemma four_list_assn_aux_append[simp]:
+  "length l1=length l1' \<Longrightarrow> 
+  length l1'=length l1'' \<Longrightarrow> 
+  length l1''=length l1''' \<Longrightarrow> 
+    four_list_assn P (l1@l2) (l1'@l2') (l1''@l2'') (l1'''@l2''')
+    = four_list_assn P l1 l1' l1'' l1''' * four_list_assn P l2 l2' l2'' l2'''"
+  apply (induct rule: list_induct4)
+  apply simp
+  apply (auto simp add: star_assoc)
+  done
+
+lemma four_list_assn_aux_ineq_len: "length l \<noteq> length l' \<or> length l' \<noteq> length l'' \<or> length l'' \<noteq> length l''' \<Longrightarrow> four_list_assn A l l' l'' l''' = false"
+proof (induction l arbitrary: l' l'' l''')
+  case (Cons x l l' l'' l''') thus ?case by (cases l'; cases l''; cases l'''; auto)
+qed auto
+
+lemma four_list_assn_aux_append2[simp]:
+  assumes "length l2=length l2'" "length l2'=length l2''" "length l2''=length l2'''" 
+    shows "four_list_assn P (l1@l2) (l1'@l2') (l1''@l2'') (l1'''@l2''')
+    = four_list_assn P l1 l1' l1'' l1''' * four_list_assn P l2 l2' l2'' l2'''"
+  apply (cases "length l1 = length l1' \<and> length l1' = length l1'' \<and> length l1'' = length l1'''")
+  subgoal by (simp; erule four_list_assn_aux_append)
+  subgoal by (simp add: four_list_assn_aux_ineq_len assms)
+  done
+
+lemma list_assn_pure_conv[constraint_simps]: "list_assn (pure R) = pure (\<langle>R\<rangle>list_rel)"
+proof (intro ext)
+  fix l li
+  show "list_assn (pure R) l li = pure (\<langle>R\<rangle>list_rel) l li"
+    apply (induction "pure R" l li rule: list_assn.induct)
+    by (auto simp: pure_def)
+qed
+
+lemmas [sepref_import_rewrite, sepref_frame_normrel_eqs, fcomp_norm_unfold] = list_assn_pure_conv[symmetric]
+
+
+lemma list_assn_simps[simp]:
+  "hn_ctxt (list_assn P) [] l' = (\<up>(l'=[]))"
+  "hn_ctxt (list_assn P) l [] = (\<up>(l=[]))"
+  "hn_ctxt (list_assn P) [] [] = emp"
+  "hn_ctxt (list_assn P) (a#as) (c#cs) = hn_ctxt P a c * hn_ctxt (list_assn P) as cs"
+  "hn_ctxt (list_assn P) (a#as) [] = false"
+  "hn_ctxt (list_assn P) [] (c#cs) = false"
+  unfolding hn_ctxt_def
+  apply (cases l')
+  apply simp
+  apply simp
+  apply (cases l)
+  apply simp
+  apply simp
+  apply simp_all
+  done
+
+lemma list_assn_precise[constraint_rules]: "precise P \<Longrightarrow> precise (list_assn P)"
+proof
+  fix l1 l2 l h F1 F2
+  assume P: "precise P"
+  assume "h\<Turnstile>list_assn P l1 l * F1 \<and>\<^sub>A list_assn P l2 l * F2"
+  thus "l1=l2"
+  proof (induct l arbitrary: l1 l2 F1 F2)
+    case Nil thus ?case by simp
+  next
+    case (Cons a ls)
+    from Cons obtain a1 ls1 where [simp]: "l1=a1#ls1"
+      by (cases l1, simp)
+    from Cons obtain a2 ls2 where [simp]: "l2=a2#ls2"
+      by (cases l2, simp)
+    
+    from Cons.prems have M:
+      "h \<Turnstile> P a1 a * list_assn P ls1 ls * F1 
+        \<and>\<^sub>A P a2 a * list_assn P ls2 ls * F2" by simp
+    have "a1=a2"
+      apply (rule preciseD[OF P, where a=a1 and a'=a2 and p=a
+        and F= "list_assn P ls1 ls * F1" 
+        and F'="list_assn P ls2 ls * F2"
+        ])
+      using M
+      by (simp add: star_assoc)
+    
+    moreover have "ls1=ls2"
+      apply (rule Cons.hyps[where ?F1.0="P a1 a * F1" and ?F2.0="P a2 a * F2"])
+      using M
+      by (simp only: star_aci)
+    ultimately show ?case by simp
+  qed
+qed
+lemma list_assn_pure[constraint_rules]: 
+  assumes P: "is_pure P" 
+  shows "is_pure (list_assn P)"
+proof -
+  from P obtain P' where P_eq: "\<And>x x'. P x x' = \<up>(P' x x')" 
+    by (rule is_pureE) blast
+
+  {
+    fix l l'
+    have "list_assn P l l' = \<up>(list_all2 P' l l')"
+      by (induct P\<equiv>P l l' rule: list_assn.induct)
+         (simp_all add: P_eq)
+  } thus ?thesis by rule
+qed
+
+lemma four_list_assn_mono: 
+  "\<lbrakk>\<And>x x' x'' x'''. P x x' x'' x'''\<Longrightarrow>\<^sub>AP' x x' x'' x'''\<rbrakk> \<Longrightarrow> four_list_assn P l l' l'' l''' \<Longrightarrow>\<^sub>A four_list_assn P' l l' l'' l'''"
+  unfolding hn_ctxt_def
+  apply (induct P l l' l'' l''' rule: four_list_assn.induct)
+  by (auto intro: ent_star_mono)
+
+lemma four_list_assn_monot: 
+  "\<lbrakk>\<And>x x' x'' x'''. P x x' x'' x'''\<Longrightarrow>\<^sub>tP' x x' x'' x'''\<rbrakk> \<Longrightarrow> four_list_assn P l l' l'' l''' \<Longrightarrow>\<^sub>t four_list_assn P' l l' l'' l'''"
+  unfolding hn_ctxt_def
+  apply (induct P l l' l'' l''' rule: four_list_assn.induct)
+  by (auto intro: entt_star_mono)
+
+lemma list_match_cong[sepref_frame_match_rules]: 
+  "\<lbrakk>\<And>x x'. \<lbrakk>x\<in>set l; x'\<in>set l'\<rbrakk> \<Longrightarrow> hn_ctxt A x x' \<Longrightarrow>\<^sub>t hn_ctxt A' x x' \<rbrakk> \<Longrightarrow> hn_ctxt (list_assn A) l l' \<Longrightarrow>\<^sub>t hn_ctxt (list_assn A') l l'"
+  unfolding hn_ctxt_def
+  by (induct A l l' rule: list_assn.induct) (simp_all add: entt_star_mono)
+
+lemma list_merge_cong[sepref_frame_merge_rules]:
+  assumes "\<And>x x'. \<lbrakk>x\<in>set l; x'\<in>set l'\<rbrakk> \<Longrightarrow> hn_ctxt A x x' \<or>\<^sub>A hn_ctxt A' x x' \<Longrightarrow>\<^sub>t hn_ctxt Am x x'"
+  shows "hn_ctxt (list_assn A) l l' \<or>\<^sub>A hn_ctxt (list_assn A') l l' \<Longrightarrow>\<^sub>t hn_ctxt (list_assn Am) l l'"
+  apply (blast intro: entt_disjE list_match_cong entt_disjD1[OF assms] entt_disjD2[OF assms])
+  done
+  
+lemma invalid_list_split: 
+  "invalid_assn (list_assn A) (x#xs) (y#ys) \<Longrightarrow>\<^sub>t invalid_assn A x y * invalid_assn (list_assn A) xs ys"
+  by (fastforce simp: invalid_assn_def intro!: enttI simp: mod_star_conv)
+
+lemma entt_invalid_list: "hn_invalid (list_assn A) l l' \<Longrightarrow>\<^sub>t hn_ctxt (list_assn (invalid_assn A)) l l'"
+  apply (induct A l l' rule: list_assn.induct)
+  applyS simp
+
+  subgoal
+    apply1 (simp add: hn_ctxt_def cong del: invalid_assn_cong)
+    apply1 (rule entt_trans[OF invalid_list_split])
+    apply (rule entt_star_mono)
+      applyS simp
+
+      apply (rule entt_trans)
+        applyS assumption
+        applyS simp
+    done
+    
+  applyS (simp add: hn_ctxt_def invalid_assn_def) 
+  applyS (simp add: hn_ctxt_def invalid_assn_def) 
+  done
+
+lemmas invalid_list_merge[sepref_frame_merge_rules] = gen_merge_cons[OF entt_invalid_list]
+
+
+lemma list_assn_comp[fcomp_norm_unfold]: "hr_comp (list_assn A) (\<langle>B\<rangle>list_rel) = list_assn (hr_comp A B)"
+proof (intro ext)  
+  { fix x l y m
+    have "hr_comp (list_assn A) (\<langle>B\<rangle>list_rel) (x # l) (y # m) = 
+      hr_comp A B x y * hr_comp (list_assn A) (\<langle>B\<rangle>list_rel) l m"
+      by (sep_auto 
+        simp: hr_comp_def list_rel_split_left_iff
+        intro!: ent_ex_preI ent_iffI) (* TODO: ent_ex_preI should be applied by default, before ent_ex_postI!*)
+  } note aux = this
+
+  fix l li
+  show "hr_comp (list_assn A) (\<langle>B\<rangle>list_rel) l li = list_assn (hr_comp A B) l li"
+    apply (induction l arbitrary: li; case_tac li; intro ent_iffI)
+    apply (sep_auto simp: hr_comp_def; fail)+
+    by (simp_all add: aux)
+qed  
+
+lemma hn_ctxt_eq: "A x y = z \<Longrightarrow> hn_ctxt A x y = z" by (simp add: hn_ctxt_def)
+
+lemmas hn_ctxt_list = hn_ctxt_eq[of "list_assn A" for A]
+
+lemma hn_case_list[sepref_prep_comb_rule, sepref_comb_rules]:
+  fixes p p' P
+  defines [simp]: "INVE \<equiv> hn_invalid (list_assn P) p p'"
+  assumes FR: "\<Gamma> \<Longrightarrow>\<^sub>t hn_ctxt (list_assn P) p p' * F"
+  assumes Rn: "p=[] \<Longrightarrow> hn_refine (hn_ctxt (list_assn P) p p' * F) f1' (hn_ctxt XX1 p p' * \<Gamma>1') R f1"
+  assumes Rs: "\<And>x l x' l'. \<lbrakk> p=x#l; p'=x'#l' \<rbrakk> \<Longrightarrow> 
+    hn_refine (hn_ctxt P x x' * hn_ctxt (list_assn P) l l' * INVE * F) (f2' x' l') (hn_ctxt P1' x x' * hn_ctxt (list_assn P2') l l' * hn_ctxt XX2 p p' * \<Gamma>2') R (f2 x l)"
+  assumes MERGE1[unfolded hn_ctxt_def]: "\<And>x x'. hn_ctxt P1' x x' \<or>\<^sub>A hn_ctxt P2' x x' \<Longrightarrow>\<^sub>t hn_ctxt P' x x'"  
+  assumes MERGE2: "\<Gamma>1' \<or>\<^sub>A \<Gamma>2' \<Longrightarrow>\<^sub>t \<Gamma>'"  
+  shows "hn_refine \<Gamma> (case_list f1' f2' p') (hn_ctxt (list_assn P') p p' * \<Gamma>') R (case_list$f1$(\<lambda>\<^sub>2x l. f2 x l)$p)"
+    apply (rule hn_refine_cons_pre[OF FR])
+    apply1 extract_hnr_invalids
+    apply (cases p; cases p'; simp add: list_assn.simps[THEN hn_ctxt_list])
+    subgoal 
+      apply (rule hn_refine_cons[OF _ Rn _ entt_refl]; assumption?)
+      applyS (simp add: hn_ctxt_def)
+
+      apply (subst mult.commute, rule entt_fr_drop)
+      apply (rule entt_trans[OF _ MERGE2])
+      apply (simp add: ent_disjI1' ent_disjI2')
+    done  
+
+    subgoal
+      apply (rule hn_refine_cons[OF _ Rs _ entt_refl]; assumption?)
+      applyS (simp add: hn_ctxt_def)
+      apply (rule entt_star_mono)
+      apply1 (rule entt_fr_drop)
+      apply (rule entt_star_mono)
+
+      apply1 (simp add: hn_ctxt_def)
+      apply1 (rule entt_trans[OF _ MERGE1])
+      applyS (simp)
+
+      apply1 (simp add: hn_ctxt_def)
+      apply (rule list_assn_monot)
+      apply1 (rule entt_trans[OF _ MERGE1])
+      applyS (simp)
+
+      apply1 (rule entt_trans[OF _ MERGE2])
+      applyS (simp)
+    done
+    done
+
+lemma hn_Nil[sepref_fr_rules]: 
+  "hn_refine emp (return []) emp (list_assn P) (RETURN$[])"
+  unfolding hn_refine_def
+  by sep_auto
+
+lemma hn_Cons[sepref_fr_rules]: "hn_refine (hn_ctxt P x x' * hn_ctxt (list_assn P) xs xs') 
+  (return (x'#xs')) (hn_invalid P x x' * hn_invalid (list_assn P) xs xs') (list_assn P)
+  (RETURN$((#) $x$xs))"
+  unfolding hn_refine_def
+  apply (sep_auto simp: hn_ctxt_def)
+  apply (rule ent_frame_fwd[OF invalidate_clone'[of P]], frame_inference)
+  apply (rule ent_frame_fwd[OF invalidate_clone'[of "list_assn P"]], frame_inference)
+  apply solve_entails
+  done
+
+lemma list_assn_aux_len: 
+  "list_assn P l l' = list_assn P l l' * \<up>(length l = length l')"
+  apply (induct P\<equiv>P l l' rule: list_assn.induct)
+  apply simp_all
+  subgoal for a as c cs
+    by (erule_tac t="list_assn P as cs" in subst[OF sym]) simp
+  done
+
+lemma list_assn_aux_eqlen_simp: 
+  "vassn_tag (list_assn P l l') \<Longrightarrow> length l' = length l"
+  "h \<Turnstile> (list_assn P l l') \<Longrightarrow> length l' = length l"
+  apply (subst (asm) list_assn_aux_len; auto simp: vassn_tag_def)+
+  done
+
+lemma hn_append[sepref_fr_rules]: "hn_refine (hn_ctxt (list_assn P) l1 l1' * hn_ctxt (list_assn P) l2 l2')
+  (return (l1'@l2')) (hn_invalid (list_assn P) l1 l1' * hn_invalid (list_assn P) l2 l2') (list_assn P)
+  (RETURN$((@) $l1$l2))"
+  apply rule
+  apply (sep_auto simp: hn_ctxt_def)
+  apply (subst list_assn_aux_len)
+  apply (sep_auto)
+  apply (rule ent_frame_fwd[OF invalidate_clone'[of "list_assn P"]], frame_inference)
+  apply (rule ent_frame_fwd[OF invalidate_clone'[of "list_assn P"]], frame_inference)
+  apply solve_entails
+  done
+
+lemma list_assn_aux_cons_conv1:
+  "list_assn R (a#l) m = (\<exists>\<^sub>Ab m'. R a b * list_assn R l m' * \<up>(m=b#m'))"
+  apply (cases m)
+  apply sep_auto
+  apply (sep_auto intro!: ent_iffI)
+  done
+lemma list_assn_aux_cons_conv2:
+  "list_assn R l (b#m) = (\<exists>\<^sub>Aa l'. R a b * list_assn R l' m * \<up>(l=a#l'))"
+  apply (cases l)
+  apply sep_auto
+  apply (sep_auto intro!: ent_iffI)
+  done
+lemmas list_assn_aux_cons_conv = list_assn_aux_cons_conv1 list_assn_aux_cons_conv2
+
+lemma list_assn_aux_append_conv1:
+  "list_assn R (l1@l2) m = (\<exists>\<^sub>Am1 m2. list_assn R l1 m1 * list_assn R l2 m2 * \<up>(m=m1@m2))"
+  apply (induction l1 arbitrary: m)
+  apply (sep_auto intro!: ent_iffI)
+  apply (sep_auto intro!: ent_iffI simp: list_assn_aux_cons_conv)
+  done
+lemma list_assn_aux_append_conv2:
+  "list_assn R l (m1@m2) = (\<exists>\<^sub>Al1 l2. list_assn R l1 m1 * list_assn R l2 m2 * \<up>(l=l1@l2))"
+  apply (induction m1 arbitrary: l)
+  apply (sep_auto intro!: ent_iffI)
+  apply (sep_auto intro!: ent_iffI simp: list_assn_aux_cons_conv)
+  done
+lemmas list_assn_aux_append_conv = list_assn_aux_append_conv1 list_assn_aux_append_conv2  
+
+declare param_upt[sepref_import_param]
+*)
+
 end
